Remove fmap (Coq has option_map). Add sections.

SysF.v
@@ -1,275 +1,316 @@
+(** Formalization of a Predicative System F
+
+We define our formalization of predicative System F by providing Coq
+datatypes for kinds, terms, types and environments. Then, we provide
+helper functions to work with these, altogether with inductive predicates
+for typing (assigning a type to a term) and kinding (assigning a kind to a
+type). *)
+
 Require Import Arith.
 
-(** A kind is entirely defined by its level in the kind hierarchy. *)
-Definition kind := nat.
+Section DataTypes.
 
-(** Inductive definition of types. *)
-Inductive typ :=
-| tvar : nat -> typ
-| tarr : typ -> typ -> typ
-| tall : kind -> typ -> typ
-.
+  (** A kind is entirely defined by its level in the kind hierarchy. *)
+  Definition kind := nat.
 
-(** Inductive definition of terms. *)
-Inductive term :=
-| var   : nat -> term
-| abs   : typ -> term -> term
-| app   : term -> term -> term
-| abs_t : kind -> term -> term
-| app_t : term -> typ -> term
-.
+  (** Inductive definition of types. *)
+  Inductive typ :=
+  | tvar : nat -> typ
+  | tarr : typ -> typ -> typ
+  | tall : kind -> typ -> typ
+  .
 
-(** [tshift X T] shifts by one the de Bruijn index of all type
-    variables in type [T] with index greater than or equal to
-    [X] at the current level. *)
-Fixpoint tshift (X : nat) (T : typ) {struct T} : typ :=
+  (** Inductive definition of terms. *)
+  Inductive term :=
+  | var   : nat -> term
+  | abs   : typ -> term -> term
+  | app   : term -> term -> term
+  | abs_t : kind -> term -> term
+  | app_t : term -> typ -> term
+  .
+
+  (** Inductive definition of environments. *)
+  Inductive env : Set :=
+  | empty : env
+  | evar  : typ -> env -> env
+  | etvar : kind -> env -> env
+  .
+
+End DataTypes.
+
+Section Equality.
+
+  Open Scope bool.
+
+  (** Structural equality over types. *)
+  Fixpoint beq_typ (T1 : typ) (T2 : typ) : bool :=
+    match (T1, T2) with
+      | (tvar X, tvar Y)           => beq_nat X Y
+      | (tarr T1 T2, tarr T1' T2') => beq_typ T1 T1' && beq_typ T2 T2'
+      | (tall K T, tall K' T')     => beq_nat K K' && beq_typ T T'
+      | _                          => false
+    end.
+
+End Equality.
+
+Section Shifting.
+
+  (** [tshift X T] shifts by one the de Bruijn index of all type
+      variables in type [T] with index greater than or equal to
+      [X] at the current level. *)
+  Fixpoint tshift (X : nat) (T : typ) {struct T} : typ :=
   match T with
   | tvar Y     => tvar (if le_gt_dec X Y then S Y else Y)
   | tarr T1 T2 => tarr (tshift X T1) (tshift X T2)
   | tall K T0  => tall K (tshift (S X) T0)
   end.
 
-(** [shift x t] shifts by one the de Bruijn index of all term
-    variables in term [t] with index greater than or equal to
-    [x] at the current level. *)
-Fixpoint shift (x : nat) (t : term) {struct t} : term :=
-  match t with
-  | var y      => var (if le_gt_dec x y then S y else y)
-  | abs T t0   => abs T (shift (S x) t0)
-  | app t1 t2  => app (shift x t1) (shift x t2)
-  | abs_t K t0 => abs_t K (shift x t0)
-  | app_t t0 T => app_t (shift x t0) T
-  end.
+  (** [shift x t] shifts by one the de Bruijn index of all term
+      variables in term [t] with index greater than or equal to
+      [x] at the current level. *)
+  Fixpoint shift (x : nat) (t : term) {struct t} : term :=
+    match t with
+      | var y      => var (if le_gt_dec x y then S y else y)
+      | abs T t0   => abs T (shift (S x) t0)
+      | app t1 t2  => app (shift x t1) (shift x t2)
+      | abs_t K t0 => abs_t K (shift x t0)
+      | app_t t0 T => app_t (shift x t0) T
+    end.
 
-(** [shift_typ X t] shifts by one the de Bruijn index of all
-    type variables in every type present in the term [t] with
-    index greater than or equal to [X] at the current level. *)
-Fixpoint shift_typ (X : nat) (t : term) {struct t} : term :=
-  match t with
-  | var y      => var y
-  | abs T t0   => abs (tshift X T) (shift_typ X t0)
-  | app t1 t2  => app (shift_typ X t1) (shift_typ X t2)
-  | abs_t K t0 => abs_t K (shift_typ (S X) t0)
-  | app_t t0 T => app_t (shift_typ X t0) (tshift X T)
-  end.
+  (** [shift_typ X t] shifts by one the de Bruijn index of all
+      type variables in every type present in the term [t] with
+      index greater than or equal to [X] at the current level. *)
+  Fixpoint shift_typ (X : nat) (t : term) {struct t} : term :=
+    match t with
+      | var y      => var y
+      | abs T t0   => abs (tshift X T) (shift_typ X t0)
+      | app t1 t2  => app (shift_typ X t1) (shift_typ X t2)
+      | abs_t K t0 => abs_t K (shift_typ (S X) t0)
+      | app_t t0 T => app_t (shift_typ X t0) (tshift X T)
+    end.
 
-(** [tsubst T X T'] replaces occurrences of the type variable
-    of de Bruijn index [X] in the type [T] by the type [T'] and
-    decreases by one the index of all type variables of greater
-    index. *)
-Fixpoint tsubst (T : typ) (X : nat) (T' : typ) {struct T} : typ :=
-  match T with
-  | tvar Y =>
-      match lt_eq_lt_dec Y X with
-      | inleft (left _)  => tvar Y
-      | inleft (right _) => T'
-      | inright _        => tvar (Y - 1)
-      end
-  | tarr T1 T2 => tarr (tsubst T1 X T') (tsubst T2 X T')
-  | tall K T0  => tall K (tsubst T0 (S X) (tshift 0 T'))
-  end.
+End Shifting.
 
-(** [subst t x t'] replaces occurrences of the variable of de Bruijn
-    index [x] in the term [t] by the term [t'] and decreases by one
-    the index of all variables of greater index. *)
-Fixpoint subst (t : term) (x : nat) (t' : term) {struct t} : term :=
-  match t with
-  | var y =>
-      match lt_eq_lt_dec y x with
-      | inleft (left _)  => var y
-      | inleft (right _) => t'
-      | inright _        => var (y - 1)
-      end
-  | abs T t0   => abs T (subst t0 (S x) (shift 0 t'))
-  | app t1 t2  => app (subst t1 x t') (subst t2 x t')
-  | abs_t K t0 => abs_t K (subst t0 x (shift_typ 0 t'))
-  | app_t t0 T => app_t (subst t0 x t') T
-  end.
+Section Substitution.
 
-(** [subst_typ t X T] replaces occurrences of the type variable of de
-    Bruijn index [X] in the term [t] by the type [T] and decreases by
-    one the index of all type variables of greater index. *)
-Fixpoint subst_typ (t : term) (X : nat) (T : typ) {struct t} : term :=
-  match t with
-  | var y       => var y
-  | abs T0 t0   => abs (tsubst T0 X T) (subst_typ t0 X T)
-  | app t1 t2   => app (subst_typ t1 X T) (subst_typ t2 X T)
-  | abs_t K t0  => abs_t K (subst_typ t0 (S X) (tshift 0 T))
-  | app_t t0 T0 => app_t (subst_typ t0 X T) (tsubst T0 X T)
-  end.
+  (** [tsubst T X T'] replaces occurrences of the type variable
+      of de Bruijn index [X] in the type [T] by the type [T'] and
+      decreases by one the index of all type variables of greater
+      index. *)
+  Fixpoint tsubst (T : typ) (X : nat) (T' : typ) {struct T} : typ :=
+    match T with
+      | tvar Y =>
+        match lt_eq_lt_dec Y X with
+          | inleft (left _)  => tvar Y
+          | inleft (right _) => T'
+          | inright _        => tvar (Y - 1)
+        end
+      | tarr T1 T2 => tarr (tsubst T1 X T') (tsubst T2 X T')
+      | tall K T0  => tall K (tsubst T0 (S X) (tshift 0 T'))
+    end.
 
-(** Inductive definition of environments. *)
-Inductive env : Set :=
-| empty : env
-| evar  : typ -> env -> env
-| etvar : kind -> env -> env
-.
+  (** [subst t x t'] replaces occurrences of the variable of de Bruijn
+      index [x] in the term [t] by the term [t'] and decreases by one
+      the index of all variables of greater index. *)
+  Fixpoint subst (t : term) (x : nat) (t' : term) {struct t} : term :=
+    match t with
+      | var y =>
+        match lt_eq_lt_dec y x with
+          | inleft (left _)  => var y
+          | inleft (right _) => t'
+          | inright _        => var (y - 1)
+        end
+      | abs T t0   => abs T (subst t0 (S x) (shift 0 t'))
+      | app t1 t2  => app (subst t1 x t') (subst t2 x t')
+      | abs_t K t0 => abs_t K (subst t0 x (shift_typ 0 t'))
+      | app_t t0 T => app_t (subst t0 x t') T
+    end.
 
-Definition fmap {A B : Type} (f : A -> B) (a : option A) :=
-  match a with
-    | None => None
-    | Some a => Some (f a)
-  end.
+  (** [subst_typ t X T] replaces occurrences of the type variable of de
+      Bruijn index [X] in the term [t] by the type [T] and decreases by
+      one the index of all type variables of greater index. *)
+  Fixpoint subst_typ (t : term) (X : nat) (T : typ) {struct t} : term :=
+    match t with
+      | var y       => var y
+      | abs T0 t0   => abs (tsubst T0 X T) (subst_typ t0 X T)
+      | app t1 t2   => app (subst_typ t1 X T) (subst_typ t2 X T)
+      | abs_t K t0  => abs_t K (subst_typ t0 (S X) (tshift 0 T))
+      | app_t t0 T0 => app_t (subst_typ t0 X T) (tsubst T0 X T)
+    end.
 
-(** [get_kind e i] returns the [i]-th kind in environment [e], if it
-    exists. *)
-Fixpoint get_kind (e : env) (i : nat) : option kind :=
-  match e with
-    | empty      => None
-    | evar _ e'  => get_kind e' i
-    | etvar K e' =>
-      match i with
-        | 0    => Some K
-        | S i' => get_kind e' i'
-      end
-  end.
+End Substitution.
 
-(** [get_typ e i] returns the [i]-th type in environment [e], if it
-    exists . *)
-Fixpoint get_typ (e : env) (i : nat) : option typ :=
-  match e with
-    | empty => None
-    | etvar _ e' => fmap (tshift 0) (get_typ e' i)
-    | evar T e' =>
-      match i with
-        | 0    => Some T
-        | S i' => get_typ e' i'
-      end
-  end.
+Section EnvironmentAccess.
 
-Open Scope bool.
+  (** [get_kind e i] returns the [i]-th kind in environment [e], if it
+      exists. *)
+  Fixpoint get_kind (e : env) (i : nat) : option kind :=
+    match e with
+      | empty      => None
+      | evar _ e'  => get_kind e' i
+      | etvar K e' =>
+        match i with
+          | 0    => Some K
+          | S i' => get_kind e' i'
+        end
+    end.
 
-Fixpoint bwf_typ (e : env) (T : typ) : bool :=
-  match T with
-    | tvar X =>
-      match get_kind e X with
-        | None => false
-        | Some _ => true
-      end
-    | tarr T1 T2 => bwf_typ e T1 && bwf_typ e T2
-    | tall K T0 => bwf_typ (etvar K e) T0
-  end.
+  (** [get_typ e i] returns the [i]-th type in environment [e], if it
+      exists. *)
+  Fixpoint get_typ (e : env) (i : nat) : option typ :=
+    match e with
+      | empty => None
+      | etvar _ e' => option_map (tshift 0) (get_typ e' i)
+      | evar T e' =>
+        match i with
+          | 0    => Some T
+          | S i' => get_typ e' i'
+        end
+    end.
 
-Fixpoint bwf_env (e : env) : bool :=
-  match e with
-    | empty      => true
-    | evar T e'  => bwf_typ e' T && bwf_env e'
-    | etvar _ e' => bwf_env e'
-  end.
+End EnvironmentAccess.
 
-Fixpoint wf_typ (e : env) (T : typ) : Prop :=
-  match T with
-    | tvar X     => get_kind e X <> None
-    | tarr T1 T2 => wf_typ e T1 /\ wf_typ e T2
-    | tall K T0  => wf_typ (etvar K e) T0
-  end.
+Section Wellformedness.
 
-Fixpoint wf_env (e : env) : Prop :=
-  match e with
-    | empty      => True
-    | evar T e'  => wf_typ e' T /\ wf_env e'
-    | etvar K e' => wf_env e'
-  end.
+  (** Wellformedness of types expressed as a logical property. *)
+  Fixpoint wf_typ (e : env) (T : typ) : Prop :=
+    match T with
+      | tvar X     => get_kind e X <> None
+      | tarr T1 T2 => wf_typ e T1 /\ wf_typ e T2
+      | tall K T0  => wf_typ (etvar K e) T0
+    end.
 
-Inductive kinding : env -> typ -> kind -> Prop :=
-| k_tvar (e : env) (X : nat) (Kp Kq : kind) :
+  (** Wellformedness of environments expressed as a logical property. *)
+  Fixpoint wf_env (e : env) : Prop :=
+    match e with
+      | empty      => True
+      | evar T e'  => wf_typ e' T /\ wf_env e'
+      | etvar K e' => wf_env e'
+    end.
+
+  Open Scope bool.
+
+  (** Wellformedness of types expressed as a decidable predicate. *)
+  Fixpoint bwf_typ (e : env) (T : typ) : bool :=
+    match T with
+      | tvar X =>
+        match get_kind e X with
+          | None   => false
+          | Some _ => true
+        end
+      | tarr T1 T2 => bwf_typ e T1 && bwf_typ e T2
+      | tall K T0  => bwf_typ (etvar K e) T0
+    end.
+
+  (** Wellformedness of environments expressed as a decidable predicate. *)
+  Fixpoint bwf_env (e : env) : bool :=
+    match e with
+      | empty      => true
+      | evar T e'  => bwf_typ e' T && bwf_env e'
+      | etvar _ e' => bwf_env e'
+    end.
+
+End Wellformedness.
+
+Section Kinding.
+
+  (** Kinding expressed as a logical property. *)
+  Inductive kinding : env -> typ -> kind -> Prop :=
+  | k_tvar (e : env) (X : nat) (Kp Kq : kind) :
       wf_env e ->
       get_kind e X = Some Kp ->
       Kp <= Kq ->
       kinding e (tvar X) Kq
-| k_tall (e : env) (T : typ) (Kp Kq : kind) :
+  | k_tall (e : env) (T : typ) (Kp Kq : kind) :
       kinding (etvar Kq e) T Kp ->
       kinding e (tall Kq T) (S (max Kp Kq))
-| k_tarr (e : env) (T1 T2 : typ) (Kp Kq : kind) :
+  | k_tarr (e : env) (T1 T2 : typ) (Kp Kq : kind) :
       kinding e T1 Kp ->
       kinding e T2 Kq ->
       kinding e (tarr T1 T2) (max Kp Kq)
-.
+  .
 
-Inductive typing : env -> term -> typ -> Prop :=
-| t_var (e : env) (X : nat) (T : typ) :
-    wf_env e ->
-    get_typ e X = Some T ->
-    typing e (var X) T
-| t_abs (e : env) (T1 T2 : typ) (t : term) :
-    wf_typ e T1 ->
-    typing (evar T1 e) t T2 ->
-    typing e (abs T1 t) (tarr T1 T2)
-| t_app (e : env) (T1 T2 : typ) (t1 : term) (t2 : term) :
-    typing e t1 (tarr T1 T2) ->
-    typing e t2 T1 ->
-    typing e (app t1 t2) T2
-| t_abs_t (e : env) (K : kind) (t : term) (T : typ) :
-    typing (etvar K e) t T ->
-    typing e (abs_t K t) (tall K T)
-| t_app_t (e : env) (K : kind) (t : term) (T1 T2 : typ) :
-    typing e t (tall K T1) ->
-    kinding e T2 K ->
-    typing e (app_t t T2) (tsubst T1 0 T2)
-.
+  (** [kind_of e T] provides a kind for type [T] in environment [e],
+      if [T] is kindable in [e]. *)
+  Fixpoint kind_of (e : env) (T : typ) : option kind :=
+    match T with
+      | tvar X => if bwf_env e then get_kind e X else None
+      | tarr T1 T2 =>
+        match kind_of e T1 with
+          | None    => None
+          | Some K1 =>
+            option_map (fun K2 => max K1 K2)
+                       (kind_of e T2)
+        end
+      | tall K T0 =>
+        option_map (fun K' => S (max K' K))
+                   (kind_of (etvar K e) T0)
+    end.
 
-Fixpoint kind_of (e : env) (T : typ) : option kind :=
-  match T with
-    | tvar X => if bwf_env e then get_kind e X else None
-    | tarr T1 T2 =>
-      match kind_of e T1 with
-        | None => None
-        | Some K1 =>
-          match kind_of e T2 with
-            | None => None
-            | Some K2 => Some (max K1 K2)
-          end
-      end
-    | tall K T0 =>
-      match kind_of (etvar K e) T0 with
-        | None => None
-        | Some K' => Some (S (max K' K))
-      end
-  end.
+End Kinding.
 
-Fixpoint beq_typ (T1 : typ) (T2 : typ) : bool :=
-  match (T1, T2) with
-    | (tvar X, tvar Y)           => beq_nat X Y
-    | (tarr T1 T2, tarr T1' T2') => beq_typ T1 T1' && beq_typ T2 T2'
-    | (tall K T, tall K' T')     => beq_nat K K' && beq_typ T T'
-    | _                          => false
-  end.
+Section Typing.
 
-Fixpoint type_of (e : env) (t : term) : option typ :=
-  match t with
-    | var x => if bwf_env e then get_typ e x else None
-    | abs T t' =>
-      match type_of (evar T e) t' with
-        | Some T' => if bwf_typ e T then Some (tarr T T') else None
-        | None => None
+  (** Typing expressed as a logical property. *)
+  Inductive typing : env -> term -> typ -> Prop :=
+  | t_var (e : env) (X : nat) (T : typ) :
+      wf_env e ->
+      get_typ e X = Some T ->
+      typing e (var X) T
+  | t_abs (e : env) (T1 T2 : typ) (t : term) :
+      wf_typ e T1 ->
+      typing (evar T1 e) t T2 ->
+      typing e (abs T1 t) (tarr T1 T2)
+  | t_app (e : env) (T1 T2 : typ) (t1 : term) (t2 : term) :
+      typing e t1 (tarr T1 T2) ->
+      typing e t2 T1 ->
+      typing e (app t1 t2) T2
+  | t_abs_t (e : env) (K : kind) (t : term) (T : typ) :
+      typing (etvar K e) t T ->
+      typing e (abs_t K t) (tall K T)
+  | t_app_t (e : env) (K : kind) (t : term) (T1 T2 : typ) :
+      typing e t (tall K T1) ->
+      kinding e T2 K ->
+      typing e (app_t t T2) (tsubst T1 0 T2)
+  .
+
+  (** [type_of e t] provides a type for term [t] in environment [e],
+      if [t] is typable in [e]. *)
+  Fixpoint type_of (e : env) (t : term) : option typ :=
+    match t with
+      | var x => if bwf_env e then get_typ e x else None
+      | abs T t' =>
+        match type_of (evar T e) t' with
+          | Some T' => if bwf_typ e T then Some (tarr T T') else None
+          | None => None
+        end
+      | app t1 t2 =>
+        match type_of e t1 with
+          | Some (tarr T1 T2) =>
+            match type_of e t2 with
+              | Some T1' =>
+                if beq_typ T1 T1'
+                then Some T2
+                else None
+              | _ => None
+            end
+          | _ => None
       end
-    | app t1 t2 =>
-      match type_of e t1 with
-        | Some (tarr T1 T2) =>
-          match type_of e t2 with
-            | Some T1' =>
-              if beq_typ T1 T1'
-              then Some T2
-              else None
-            | _ => None
-          end
-        | _ => None
-      end
-    | abs_t K t' =>
-      match type_of (etvar K e) t' with
-        | Some T => Some (tall K T)
-        | None => None
-      end
-    | app_t t' T =>
-      match type_of e t' with
-        | Some (tall K T') =>
-          match kind_of e T with
-            | Some K' =>
-              if leb K' K
-              then Some (tsubst T' 0 T)
-              else None
-            | None => None
-          end
-        | _ => None
-      end
-  end.
+      | abs_t K t' =>
+        option_map (fun T => tall K T)
+                   (type_of (etvar K e) t')
+      | app_t t' T =>
+        match type_of e t' with
+          | Some (tall K T') =>
+            match kind_of e T with
+              | Some K' =>
+                if leb K' K
+                then Some (tsubst T' 0 T)
+                else None
+              | None => None
+            end
+          | _ => None
+        end
+    end.
+
+End Typing.
